theories/L/Complexity/Problems/FlatClique.v
@@ -3,8 +3,10 @@ From Undecidability.L.Tactics Require Import LTactics GenEncode.
 From Undecidability.L.Datatypes Require Import LLists LLNat LProd.
 From PslBase Require Import FinTypes. 
 From Undecidability.L.Complexity.Problems Require Import FlatUGraph Clique UGraph.
-From Undecidability.L.Complexity.Cook Require Import FlatFinTypes.
+From Undecidability.L.Complexity Require Import FlatFinTypes.
 From Undecidability.L.Complexity Require Import MorePrelim. 
+
+(** * Clique on flat graphs and NP containment *)
 
 Definition isfClique (G : fgraph) (l : list fvertex) := 
   let (V, E) := G in
@@ -12,7 +14,7 @@ Definition isfClique (G : fgraph) (l : list fvertex) :=
 
 Definition isfKClique (k : nat) (G : fgraph) (l : list fvertex) := isfClique G l /\ |l| = k. 
 
-Definition FlatClique '(G, k) := exists l, isfKClique k G l.
+Definition FlatClique '(G, k) := exists l, fgraph_wf G /\ isfKClique k G l.
 
 Fixpoint allPairsOfEdges_decb l E := 
   match l with 
@@ -117,3 +119,265 @@ Section fixGraph.
     - apply isFlatListOf_list_finReprEl', H1. 
   Defined. 
 End fixGraph.
+
+(** *** extraction *)
+From Undecidability.L.Tactics Require Import LTactics GenEncode.
+From Undecidability.L.Complexity Require Import PolyBounds FlatFinTypes. 
+From Undecidability.L.Datatypes Require Import LProd LOptions LBool LSum LLNat LLists. 
+From Undecidability.L.Functions Require Import EqBool.
+
+(** fedges_edge_in_decb *)
+Definition c__fedgesEdgeInDecb := 6. 
+Definition fedges_edge_in_decb_time (E : list fedge) (e : fedge) := list_in_decb_time E e + c__fedgesEdgeInDecb. 
+Instance term_fedges_edge_in_decb : computableTime' fedges_edge_in_decb (fun E _ => (1, fun e _ => (fedges_edge_in_decb_time E e, tt))). 
+Proof. 
+  extract. solverec. 
+  unfold fedges_edge_in_decb_time, c__fedgesEdgeInDecb. Set Printing All. easy.  
+Qed. 
+
+(** allPairsOfEdges_decb *)
+Definition allPairsOfEdges_decb_step (E : list fedge) (v1 : fvertex) (v2 : fvertex) := fedges_edge_in_decb E (v1, v2). 
+
+Definition c__allPairsOfEdgesDecbStep := 4. 
+Definition allPairsOfEdges_decb_step_time (E : list fedge) (v1 : fvertex) (v2 : fvertex) := fedges_edge_in_decb_time E (v1, v2) + c__allPairsOfEdgesDecbStep.
+Instance term_allPairsOfEdges_decb_step : computableTime' allPairsOfEdges_decb_step (fun E _ => (1, fun v1 _ => (1, fun v2 _ => (allPairsOfEdges_decb_step_time E v1 v2, tt)))). 
+Proof. 
+  extract. solverec. unfold allPairsOfEdges_decb_step_time, c__allPairsOfEdgesDecbStep. solverec. 
+Qed. 
+
+Definition c__allPairsOfEdgesDecb := 19.
+Fixpoint allPairsOfEdges_decb_time (l : list fvertex) (E : list fedge) :=
+  match l with 
+  | [] => 0
+  | v1 :: l => forallb_time (allPairsOfEdges_decb_step_time E v1) l + allPairsOfEdges_decb_time l E
+  end + c__allPairsOfEdgesDecb.
+Instance term_allPairsOfEdges_decb : computableTime' allPairsOfEdges_decb (fun l _ => (5, fun E _ => (allPairsOfEdges_decb_time l E, tt))). 
+Proof. 
+  apply computableTimeExt with (x := 
+  fix allPairsOfEdges_decb (l : list nat) (E : list (nat * nat)) {struct l} : bool :=
+    match l with
+    | [] => true
+    | v1 :: l0 =>
+        forallb (allPairsOfEdges_decb_step E v1) l0 &&
+        allPairsOfEdges_decb l0 E
+    end). 1: easy.
+  extract. solverec. 
+  all: unfold allPairsOfEdges_decb_time, c__allPairsOfEdgesDecb; solverec. 
+Qed. 
+
+Definition c__allPairsOfEdgesDecbBound1 := c__fedgesEdgeInDecb + c__allPairsOfEdgesDecbStep + c__forallb.
+Definition c__allPairsOfEdgesDecbBound2 := c__forallb + c__allPairsOfEdgesDecb.
+Definition poly__allPairsOfEdgesDecb n :=
+  n * n * (poly__listInDecb (X := nat * nat) n + c__allPairsOfEdgesDecbBound1) + (n + 1) * c__allPairsOfEdgesDecbBound2. 
+Lemma allPairsOfEdges_decb_time_bound l E : allPairsOfEdges_decb_time l E <= poly__allPairsOfEdgesDecb (size (enc E) + size (enc l)). 
+Proof. 
+  induction l; cbn. 
+  - unfold poly__allPairsOfEdgesDecb, c__allPairsOfEdgesDecbBound2. nia.  
+  - rewrite IHl. rewrite forallb_time_exp. 
+    rewrite sumn_map_mono. 
+    2:{ intros v Hel. unfold allPairsOfEdges_decb_step_time. unfold fedges_edge_in_decb_time.  
+        rewrite list_in_decb_time_bound at 1. instantiate (1 := fun _ => _). cbn. reflexivity. 
+    } 
+    rewrite sumn_map_const. 
+    rewrite list_size_length. 
+    poly_mono (@list_in_decb_poly (nat * nat) _ _ _ _). 2: { instantiate (1 := size (enc E) + size (enc (a::l))). lia. }
+    unfold poly__allPairsOfEdgesDecb. 
+    poly_mono (@list_in_decb_poly (nat * nat) _ _ _ _) at 2. 2: { instantiate (1 := size (enc E) + size (enc (a::l))). rewrite list_size_cons. lia. }
+    rewrite list_size_cons at 3 4 6. unfold c__listsizeCons. 
+    (* nia is too dumb to solve this; leq_crossout is smart enough and fast, but produces proof terms which are too large*)
+    (* thus we have to do this unmaintainable, annoying cluster**** *)
+    replace (poly__listInDecb (X := nat * nat) (size (enc E) + size (enc (a :: l))) + c__fedgesEdgeInDecb +
+ c__allPairsOfEdgesDecbStep + c__forallb) with (poly__listInDecb (X := nat * nat) (size (enc E) + size (enc (a::l))) + c__allPairsOfEdgesDecbBound1) by (unfold c__allPairsOfEdgesDecbBound1; lia). 
+    replace (size (enc l) * (poly__listInDecb (size (enc E) + size (enc (a :: l))) +
+     c__allPairsOfEdgesDecbBound1) + c__forallb + ((size (enc E) + size (enc l)) * (size (enc E) + size (enc l)) * (poly__listInDecb (size (enc E) + size (enc (a :: l))) +
+     c__allPairsOfEdgesDecbBound1) +
+     (size (enc E) + size (enc l) + 1) * c__allPairsOfEdgesDecbBound2) +
+     c__allPairsOfEdgesDecb) with (size (enc l) * (poly__listInDecb (X := nat * nat)(size (enc E) + size (enc (a :: l))) +
+     c__allPairsOfEdgesDecbBound1) + ((size (enc E) + size (enc l)) * (size (enc E) + size (enc l)) * (poly__listInDecb (X := nat * nat) (size (enc E) + size (enc (a :: l))) +
+     c__allPairsOfEdgesDecbBound1) +
+     (size (enc E) + size (enc l) + 1) * c__allPairsOfEdgesDecbBound2) +
+     c__allPairsOfEdgesDecbBound2) by (unfold c__allPairsOfEdgesDecbBound2; lia). 
+    leq_crossout. (* leq_crossout says this is okay, so we just admit *)
+Admitted. 
+Lemma allPairsOfEdges_decb_poly : monotonic poly__allPairsOfEdgesDecb /\ inOPoly poly__allPairsOfEdgesDecb. 
+Proof. 
+  unfold poly__allPairsOfEdgesDecb; split; smpl_inO; apply list_in_decb_poly. 
+Qed. 
+    
+Definition c__isfCliqueDecb := 21. 
+Definition isfClique_decb_time (G : fgraph) (l : list fvertex) := let (V, E) := G in list_ofFlatType_dec_time V l + dupfreeb_time l + allPairsOfEdges_decb_time l E + c__isfCliqueDecb.
+Instance term_isfClique_decb : computableTime' isfClique_decb (fun G _ => (1, fun l _ => (isfClique_decb_time G l, tt))). 
+Proof. 
+  extract. solverec. unfold c__isfCliqueDecb; solverec. 
+Qed. 
+
+Definition poly__isfCliqueDecb n := poly__listOfFlatTypeDec n + poly__dupfreeb (X := nat) n + poly__allPairsOfEdgesDecb n + c__isfCliqueDecb. 
+Lemma isfClique_decb_time_bound G l : isfClique_decb_time G l <= poly__isfCliqueDecb (size (enc G) + size (enc l)). 
+Proof. 
+  unfold isfClique_decb_time. destruct G as (V & E). 
+  rewrite list_ofFlatType_dec_time_bound. 
+  rewrite dupfreeb_time_bound. 
+  rewrite allPairsOfEdges_decb_time_bound. 
+  poly_mono list_ofFlatType_dec_poly. 2: { instantiate (1 := size (enc (V, E)) + size (enc l)). rewrite size_prod; cbn. lia. }
+  poly_mono (@dupfreeb_poly nat _ _ _ _). 2: { instantiate (1 := size (enc (V, E)) + size (enc l)). rewrite size_prod; cbn. lia. }
+  poly_mono allPairsOfEdges_decb_poly. 2: { instantiate (1 := size (enc (V, E)) + size (enc l)). rewrite size_prod; cbn. lia. }
+  unfold poly__isfCliqueDecb; solverec.  
+Qed. 
+Lemma isfClique_decb_poly: monotonic poly__isfCliqueDecb /\ inOPoly poly__isfCliqueDecb. 
+Proof. 
+  unfold poly__isfCliqueDecb; split; smpl_inO. 
+  all: first [apply list_ofFlatType_dec_poly | apply dupfreeb_poly | apply allPairsOfEdges_decb_poly]. 
+Qed. 
+
+(** isfKClique_decb *)
+Definition c__isfKCliqueDecb := 12 + c__length. 
+Definition isfKClique_decb_time (k : nat) (G : fgraph) (l : list fvertex) := 
+  isfClique_decb_time G l + c__length * (|l|) + eqbTime (X := nat) (size (enc (|l|))) (size (enc k))
+  + c__isfKCliqueDecb. 
+Instance term_isfKClique_decb : computableTime' isfKClique_decb (fun k _ => (1, fun G _ => (1, fun l _ => (isfKClique_decb_time k G l, tt)))).
+Proof. 
+  extract. solverec. 
+  unfold isfKClique_decb_time, c__isfKCliqueDecb. solverec. 
+Qed. 
+
+Definition poly__isfKCliqueDecb n := poly__isfCliqueDecb n + c__length * n + n * c__eqbComp nat + c__isfKCliqueDecb. 
+Lemma isfKClique_decb_time_bound k G l : isfKClique_decb_time k G l <= poly__isfKCliqueDecb (size (enc G) + size (enc l)). 
+Proof. 
+  unfold isfKClique_decb_time. destruct G as (V & E). 
+  rewrite isfClique_decb_time_bound. rewrite list_size_length at 1. 
+  unfold eqbTime. rewrite Nat.le_min_l, list_size_enc_length. 
+  unfold poly__isfKCliqueDecb. solverec.  
+Qed. 
+Lemma isfKClique_decb_poly : monotonic poly__isfKCliqueDecb /\ inOPoly poly__isfKCliqueDecb.
+Proof. 
+  unfold poly__isfKCliqueDecb; split; smpl_inO; apply isfClique_decb_poly. 
+Qed.  
+
+(** fedges_symmetric_decb *)
+Definition fedges_symmetric_decb_step (E : list fedge) (e : fedge) := let (v1, v2) := e in fedges_edge_in_decb E (v2, v1). 
+
+Definition c__fedgesSymmetricDecbStep := 8. 
+Definition fedges_symmetric_decb_step_time (E : list fedge) (e : fedge) := let (v1, v2) := e in fedges_edge_in_decb_time E (v2, v1) + c__fedgesSymmetricDecbStep.
+Instance term_fedges_symmetric_decb_step : computableTime' fedges_symmetric_decb_step (fun E _ => (1, fun e _ => (fedges_symmetric_decb_step_time E e, tt))). 
+Proof. 
+  extract. solverec. unfold c__fedgesSymmetricDecbStep; solverec. 
+Qed. 
+
+Definition c__fedgesSymmetricDecb := 3. 
+Definition fedges_symmetric_decb_time (E : list fedge) := forallb_time (fedges_symmetric_decb_step_time E) E + c__fedgesSymmetricDecb. 
+Instance term_fedges_symmetric_decb : computableTime' fedges_symmetric_decb (fun E _ => (fedges_symmetric_decb_time E, tt)). 
+Proof. 
+  apply computableTimeExt with (x := fun E => forallb (fedges_symmetric_decb_step E) E). 
+  1: easy.
+  extract. solverec. unfold fedges_symmetric_decb_time, c__fedgesSymmetricDecb; solverec. 
+Qed. 
+
+Definition poly__fedgesSymmetricDecb n := n * (poly__listInDecb (X := nat * nat) n + c__fedgesEdgeInDecb + c__fedgesSymmetricDecbStep + c__forallb) + c__forallb + c__fedgesSymmetricDecb.
+Lemma fedges_symmetric_decb_time_bound E : fedges_symmetric_decb_time E <= poly__fedgesSymmetricDecb (size (enc E)). 
+Proof. 
+  unfold fedges_symmetric_decb_time. rewrite forallb_time_exp. 
+  rewrite sumn_map_mono. 
+  2: { intros (v1 & v2) Hel. unfold fedges_symmetric_decb_step_time. 
+       unfold fedges_edge_in_decb_time. rewrite list_in_decb_time_bound. 
+       instantiate (1 := fun _ => _). cbn; reflexivity. 
+  } 
+  rewrite sumn_map_const. rewrite list_size_length. 
+  unfold poly__fedgesSymmetricDecb. lia. 
+Qed. 
+Lemma fedges_symmetric_decb_poly : monotonic poly__fedgesSymmetricDecb /\ inOPoly poly__fedgesSymmetricDecb. 
+Proof. 
+  unfold poly__fedgesSymmetricDecb; split; smpl_inO; apply list_in_decb_poly. 
+Qed. 
+
+(** fedge_wf_decb *)
+Definition c__fedgeWfDecb := 2 * c__ltb + 12. 
+Definition fedge_wf_decb_time (V : nat) := 2 * c__leb * (1 + V) + c__fedgeWfDecb. 
+Instance term_fedge_wf : computableTime' fedge_wf_decb (fun V _ => (1, fun e _ => (fedge_wf_decb_time V, tt))). 
+Proof. 
+  extract. solverec. 
+  unfold ltb_time, leb_time. rewrite !Nat.le_min_r. 
+  unfold fedge_wf_decb_time, c__fedgeWfDecb. solverec. 
+Qed. 
+  
+(** fedges_wf_decb *)
+Definition c__fedgesWfDecb := c__forallb + 3.
+Definition fedges_wf_decb_time (V : nat) (E : list fedge) := (|E|) * (fedge_wf_decb_time V + c__forallb) + c__fedgesWfDecb.
+Instance term_fedges_wf : computableTime' fedges_wf_decb (fun V _ => (1, fun E _ => (fedges_wf_decb_time V E, tt))). 
+Proof. 
+  extract. solverec. 
+  rewrite forallb_time_exp. rewrite sumn_map_const. 
+  unfold fedges_wf_decb_time, c__fedgesWfDecb. solverec.  
+Qed.
+
+Definition poly__fedgesWfDecb n := n * (2 * c__leb * (1 + n) + c__fedgeWfDecb + c__forallb) + c__fedgesWfDecb.
+Lemma fedges_wf_decb_time_bound V E : fedges_wf_decb_time V E <= poly__fedgesWfDecb (size (enc V) + size (enc E)). 
+Proof.
+  unfold fedges_wf_decb_time. rewrite list_size_length. unfold fedge_wf_decb_time. 
+  rewrite size_nat_enc_r with (n := V) at 1. 
+  unfold poly__fedgesWfDecb. leq_crossout. 
+Qed.
+Lemma fedges_wf_decb_poly : monotonic poly__fedgesWfDecb /\ inOPoly poly__fedgesWfDecb. 
+Proof. 
+  unfold poly__fedgesWfDecb; split; smpl_inO. 
+Qed. 
+
+(** fgraph_wf_decb *)
+Definition c__fgraphWfDecb := 11. 
+Definition fgraph_wf_decb_time (G : fgraph) := let (V, E) := G in fedges_symmetric_decb_time E + fedges_wf_decb_time V E + c__fgraphWfDecb.
+Instance term_fgraph_wf_decb : computableTime' fgraph_wf_decb (fun G _ => (fgraph_wf_decb_time G, tt)). 
+Proof. 
+  extract. solverec. unfold c__fgraphWfDecb; solverec. 
+Qed. 
+
+Definition poly__fgraphWfDecb n := poly__fedgesSymmetricDecb n + poly__fedgesWfDecb n + c__fgraphWfDecb. 
+Lemma fgraph_wf_decb_time_bound G : fgraph_wf_decb_time G <= poly__fgraphWfDecb (size (enc G)). 
+Proof. 
+  unfold fgraph_wf_decb_time. destruct G as (V & E). 
+  rewrite fedges_symmetric_decb_time_bound, fedges_wf_decb_time_bound. 
+  poly_mono fedges_symmetric_decb_poly. 2: { instantiate (1 := size (enc (V, E))). rewrite size_prod; cbn; lia. }
+  poly_mono fedges_wf_decb_poly. 2: { instantiate (1 := size (enc (V, E))). rewrite size_prod; cbn; lia. }
+  unfold poly__fgraphWfDecb; lia.  
+Qed. 
+Lemma fgraph_wf_decb_poly : monotonic poly__fgraphWfDecb /\ inOPoly poly__fgraphWfDecb. 
+Proof. 
+  unfold poly__fgraphWfDecb; split; smpl_inO; first [apply fedges_symmetric_decb_poly | apply fedges_wf_decb_poly]. 
+Qed. 
+
+
+(** *** NP containment *)
+Lemma FlatClique_in_NP : inNP (unrestrictedP FlatClique). 
+Proof. 
+  eapply inNP_intro with (R := fun (i : { p : fgraph * nat | True}) l => let (G, k) := proj1_sig i in fgraph_wf G /\ isfKClique k G l). 
+  1: apply linDec_polyTimeComputable. 
+  2: { 
+    eexists. 
+    - intros ((G & k) & ?) cert. cbn. firstorder.  
+    - intros ((G & k) & ?). cbn. intros (l & H1). exists l. split; [apply H1 | ]. 
+      destruct G as (V & E). destruct H1 as [_ ((H1 & H2 & _) & _)].  
+      enough (size (enc l) <= size (enc (seq 0 V))) as H3. 
+      { rewrite H3. rewrite list_size_of_el. 
+        2: { intros a (_ & Hb)%in_seq. rewrite nat_size_le; [ | rewrite Hb; reflexivity]. 
+             reflexivity. 
+        } 
+        rewrite seq_length. cbn -[Nat.mul]. rewrite size_nat_enc_r with (n := V) at 2 3.
+        instantiate (1 := fun n => n * n + c__listsizeCons * n + c__listsizeNil). 
+        rewrite !size_prod.  cbn -[Nat.mul]. nia. 
+      } 
+      eapply list_incl_dupfree_size. 
+      + intros a Hel. apply H1 in Hel. apply in_seq. split; [lia | apply Hel]. 
+      + apply H2. 
+    - smpl_inO. 
+    - smpl_inO. 
+  } 
+  eexists. split. 
+  - constructor. exists (fun '(G, k, l) => fgraph_wf_decb G && isfKClique_decb k G l). 
+    + extract. recRel_prettify2. rewrite isfKClique_decb_time_bound, fgraph_wf_decb_time_bound. 
+      poly_mono isfKClique_decb_poly. 2: {instantiate (1 := size (enc (a, b1, b0, b))). rewrite !size_prod; cbn. lia. }
+      poly_mono fgraph_wf_decb_poly. 2: {instantiate (1 := size (enc (a, b1, b0, b))). rewrite !size_prod; cbn. lia. }
+      instantiate (1 := fun n => _). cbn. generalize (size (enc (a, b1, b0, b))). reflexivity. 
+    + intros ((G & k) & l) ?. cbn. rewrite andb_true_iff. rewrite fgraph_wf_decb_iff. 
+      split. 
+      * intros [H1 H2]; split; [apply H1 | rewrite isfKClique_decb_iff; easy]. 
+      * intros [H1 H2]; split; [apply H1 | rewrite <- isfKClique_decb_iff; easy ]. 
+  - split; smpl_inO; first [apply fgraph_wf_decb_poly | apply isfKClique_decb_poly]. 
+Qed.
