theories/L/Complexity/Cook/FlatTPR.v
@@ -1,4 +1,4 @@
-From Undecidability.L.Complexity.Cook Require Import Prelim FlatPR FlatFinTypes. 
+From Undecidability.L.Complexity Require Import MorePrelim Cook.FlatPR FlatFinTypes. 
 From Undecidability.L.Complexity.Cook Require Export TPR.
 From PslBase Require Import Base FinTypes. 
 Require Import Lia.
