theories/L/Complexity/Cook/FlatTPR_to_FlatPR.v
@@ -1,6 +1,6 @@
 From PslBase Require Import Base FinTypes. 
 From PslBase Require Import Vectors.Vectors. 
-From Undecidability Require Import L.Complexity.Cook.Prelim FlatTPR FlatPR TPR_to_PR.
+From Undecidability.L.Complexity Require Import MorePrelim Cook.FlatTPR Cook.FlatPR Cook.TPR_to_PR.
 Require Import Lia.
 
 (** *Reduction of FlatTPR to FlatPR*)
