theories/L/Complexity/Cook/UniformHomomorphisms.v
@@ -1,5 +1,5 @@
 From PslBase Require Import Base FiniteTypes. 
-From Undecidability.L.Complexity.Cook Require Import Prelim.
+From Undecidability.L.Complexity Require Import MorePrelim.
 Require Import Lia.
 
 (** * Uniform homomorphisms *)
